SSA/Experimental/Bits/Fast/Circuit.lean
@@ -13,8 +13,7 @@ to the arity of `α`. See also `eval` for the explicit conversion of a circuit t
 inductive Circuit (α : Type u) : Type u
   | tru : Circuit α
   | fals : Circuit α
-  /-- `var b x` represents literal `x` or the negated literat `¬x`,
-      depending on the value of `b` -/
+  /-- `var b x` represents literal `x` if `b = true` or the negated literat `¬x` if `b = false` -/
   | var : Bool → α → Circuit α
   | and : Circuit α → Circuit α → Circuit α
   | or : Circuit α → Circuit α → Circuit α
